src/example/LockClientW.v
@@ -97,7 +97,7 @@ End ClientSpec.
 
 
 From Fairness Require Import
-     IProp IPM Weakest ModSim PCM MonotonePCM StateRA FairRA NatStructs NatMapRA.
+     IProp IPMFOS Weakest ModSim PCMFOS MonotonePCM StateRA FairRA NatStructs NatMapRAFOS.
 
 Section LEMMA.
 
@@ -151,7 +151,7 @@ Section SIM.
   Context `{AUTHNRA: @GRA.inG (Auth.t (Excl.t nat)) Σ}.
   Context `{AUTHVWRA: @GRA.inG (Auth.t (Excl.t View.t)) Σ}.
   Context `{AUTHVWRA2: @GRA.inG (Auth.t (Excl.t (View.t * unit))) Σ}.
-  Context `{AUTHNMNRA: @GRA.inG (Auth.t (NatMapRA.t nat)) Σ}.
+  Context `{AUTHNMNRA: @GRA.inG (Auth.t (NatMapRAFOS.t nat)) Σ}.
 
   Definition thread1_will_write (tvw: View.t) : iProp :=
     ∃ k, (∃ n, ObligationRA.black k n)
@@ -168,7 +168,7 @@ Section SIM.
 
   Definition lock_will_unlock : iProp :=
     ∃ (own: bool) (tvw: View.t) (ing: bool) (mem: WMem.t) (wobl: NatMap.t nat) (j: nat),
-      (OwnM (Auth.black (Some wobl: NatMapRA.t nat)))
+      (OwnM (Auth.black (Some wobl: NatMapRAFOS.t nat)))
         ∗
         ((OwnM (Auth.black (Excl.just j: Excl.t nat)))
         ∗ (OwnM (Auth.black (Excl.just (tvw, tt): Excl.t (View.t * unit)%type))))
@@ -234,7 +234,7 @@ Section SIM.
         (
             OwnM (OneShot.pending nat 1)
         ) ∗ (
-            OwnM (Auth.black (Some (NatMap.empty nat) : NatMapRA.t nat))
+            OwnM (Auth.black (Some (NatMap.empty nat) : NatMapRAFOS.t nat))
               ∗ OwnM (Auth.black (Excl.just 0 : Excl.t nat))
               ∗ OwnM (Auth.white (Excl.just 0 : Excl.t nat))
               ∗ OwnM (Auth.black (Excl.just View.bot : Excl.t View.t))
@@ -365,7 +365,7 @@ Section SIM.
 
     Definition lock_will_unlock : iProp :=
       ∃ (own: bool) (tvw: View.t) (ing: bool) (mem: WMem.t) (wobl: NatMap.t nat) (j: nat),
-        (OwnM (Auth.black (Some wobl: NatMapRA.t nat)))
+        (OwnM (Auth.black (Some wobl: NatMapRAFOS.t nat)))
           ∗
           ((OwnM (Auth.black (Excl.just j: Excl.t nat)))
           ∗ (OwnM (Auth.black (Excl.just (tvw, tt): Excl.t (View.t * unit)%type))))
@@ -535,8 +535,8 @@ Section SIM.
 
     (* make (Auth.white singleton tid k) and update wobl *)
     iPoseProof (OwnM_Upd with "B1") as "OWN1".
-    { eapply Auth.auth_alloc. instantiate (1:=NatMapRA.singleton tid k).
-      instantiate (1:=Some (NatMap.add tid k wobl)). eapply NatMapRA.add_local_update.
+    { eapply Auth.auth_alloc. instantiate (1:=NatMapRAFOS.singleton tid k).
+      instantiate (1:=Some (NatMap.add tid k wobl)). eapply NatMapRAFOS.add_local_update.
       eapply NatMapP.F.not_find_in_iff; auto.
     }
     iMod "OWN1" as "[OWNB1 MYSING]".
@@ -613,8 +613,8 @@ Section SIM.
 
       iAssert (⌜NatMap.find tid wobl = Some k⌝)%I as "%".
       { iPoseProof (OwnM_valid with "[MYW B1]") as "%".
-        { instantiate (1:= (Auth.black (Some wobl: NatMapRA.t nat)) ⋅ (Auth.white (NatMapRA.singleton tid k: NatMapRA.t nat))). iSplitL "B1"; iFrame. }
-        eapply Auth.auth_included in H. eapply NatMapRA.extends_singleton_iff in H.
+        { instantiate (1:= (Auth.black (Some wobl: NatMapRAFOS.t nat)) ⋅ (Auth.white (NatMapRAFOS.singleton tid k: NatMapRAFOS.t nat))). iSplitL "B1"; iFrame. }
+        eapply Auth.auth_included in H. eapply NatMapRAFOS.extends_singleton_iff in H.
         auto.
       }
       rename H into FIND.
@@ -665,8 +665,8 @@ Section SIM.
 
       iAssert (⌜NatMap.find tid wobl = Some k⌝)%I as "%".
       { iPoseProof (OwnM_valid with "[MYW B1]") as "%".
-        { instantiate (1:= (Auth.black (Some wobl: NatMapRA.t nat)) ⋅ (Auth.white (NatMapRA.singleton tid k: NatMapRA.t nat))). iSplitL "B1"; iFrame. }
-        eapply Auth.auth_included in H. eapply NatMapRA.extends_singleton_iff in H.
+        { instantiate (1:= (Auth.black (Some wobl: NatMapRAFOS.t nat)) ⋅ (Auth.white (NatMapRAFOS.singleton tid k: NatMapRAFOS.t nat))). iSplitL "B1"; iFrame. }
+        eapply Auth.auth_included in H. eapply NatMapRAFOS.extends_singleton_iff in H.
         auto.
       }
       rename H into FIND.
@@ -695,8 +695,8 @@ Section SIM.
 
       (* close invariant *)
       iPoseProof (OwnM_Upd with "[B1 MYW]") as "> B1".
-      2:{ instantiate (1:= (Auth.black (Some wobl: NatMapRA.t nat)) ⋅ (Auth.white (NatMapRA.singleton tid k: NatMapRA.t nat))). iSplitL "B1"; iFrame. }
-      { eapply Auth.auth_dealloc. eapply NatMapRA.remove_local_update. }
+      2:{ instantiate (1:= (Auth.black (Some wobl: NatMapRAFOS.t nat)) ⋅ (Auth.white (NatMapRAFOS.singleton tid k: NatMapRAFOS.t nat))). iSplitL "B1"; iFrame. }
+      { eapply Auth.auth_dealloc. eapply NatMapRAFOS.remove_local_update. }
       rewrite <- key_set_pull_rm_eq in *. remember (NatMap.remove tid wobl) as new_wobl.
 
       iPoseProof (MonotonePCM.list_prop_sum_cons_unfold with "MYDUTY") as "[MYDUTY _]".
@@ -1374,7 +1374,7 @@ Module LockClientWCorrect.
                  (Auth.t (Excl.t nat));
                  (Auth.t (Excl.t View.t));
                  (Auth.t (Excl.t (View.t * unit)));
-                 (Auth.t (NatMapRA.t nat));
+                 (Auth.t (NatMapRAFOS.t nat));
                  CoPset.t;
                  Gset.t;
                  InvSetRA (Prop)
@@ -1401,7 +1401,7 @@ Module LockClientWCorrect.
   Local Instance AUTHNRA: @GRA.inG (Auth.t (Excl.t nat)) Σ := (@GRA.InG _ _ 16 (@eq_refl _ _)).
   Local Instance AUTHVWRA: @GRA.inG (Auth.t (Excl.t View.t)) Σ := (@GRA.InG _ _ 17 (@eq_refl _ _)).
   Local Instance AUTHVWRA2: @GRA.inG (Auth.t (Excl.t (View.t * unit))) Σ := (@GRA.InG _ _ 18 (@eq_refl _ _)).
-  Local Instance AUTHNMNRA: @GRA.inG (Auth.t (NatMapRA.t nat)) Σ := (@GRA.InG _ _ 19 (@eq_refl _ _)).
+  Local Instance AUTHNMNRA: @GRA.inG (Auth.t (NatMapRAFOS.t nat)) Σ := (@GRA.InG _ _ 19 (@eq_refl _ _)).
 
   Local Instance COPSETRA: @GRA.inG CoPset.t Σ := (@GRA.InG _ _ 20 (@eq_refl _ _)).
   Local Instance GSETRA : @GRA.inG Gset.t Σ := (@GRA.InG _ _ 21 (@eq_refl _ _)).
@@ -1417,7 +1417,7 @@ Module LockClientWCorrect.
 
   Let init_res :=
         (GRA.embed (OneShot.pending nat 1))
-          ⋅ GRA.embed (Auth.black (Some (NatMap.empty nat) : NatMapRA.t nat))
+          ⋅ GRA.embed (Auth.black (Some (NatMap.empty nat) : NatMapRAFOS.t nat))
           ⋅ GRA.embed (Auth.black (Excl.just 0 : Excl.t nat) ⋅ Auth.white (Excl.just 0 : Excl.t nat))
           ⋅ GRA.embed (Auth.black (Excl.just View.bot : Excl.t View.t) ⋅ Auth.white (Excl.just View.bot : Excl.t View.t))
           ⋅ GRA.embed (Auth.black (Excl.just (View.bot, ()) : Excl.t (View.t * unit))
